Port the soundness proof for backtracker

regex/Regex/Backtracker/Basic.lean
@@ -88,11 +88,6 @@ where
   termination_by bit.remainingBytes
 
 def captureNextBuf (nfa : NFA) (wf : nfa.WellFormed) (bufferSize : Nat) (it : Iterator) : Option (Buffer bufferSize) :=
-  let _ := BufferStrategy bufferSize
   captureNext (BufferStrategy bufferSize) nfa wf it
-
-def searchNext (nfa : NFA) (wf : nfa.WellFormed) (it : Iterator) : Option (Pos × Pos) := do
-  let slots ← captureNextBuf nfa wf 2 it
-  pure (← slots[0], ← slots[1])
 
 end Regex.Backtracker
