correctness/RegexCorrectness/Backtracker/Correctness.lean
@@ -12,16 +12,19 @@ namespace Regex.Backtracker
 theorem captureNext_correct {e bufferSize it matchedB}
   (disj : e.Disjoint)
   (hresB : captureNext (BufferStrategy bufferSize) (NFA.compile e) NFA.compile_wf it = .some matchedB) (v : it.Valid) :
-  ∃ l r span groups,
-    span.toString = it.toString ∧
-    e.Captures ⟨l, [], r⟩ span groups ∧
+  ∃ l m r groups,
+    it.toString = ⟨l ++ m ++ r⟩ ∧
+    e.Captures ⟨l, [], m ++ r⟩ ⟨l, m.reverse, r⟩ groups ∧
     EquivMaterializedUpdate (materializeRegexGroups groups) matchedB := by
   match hresH : captureNext HistoryStrategy (NFA.compile e) NFA.compile_wf it with
   | .some matchedH =>
     have ref := hresH ▸ hresB ▸ captureNext.refines (NFA.compile e) NFA.compile_wf bufferSize it
     simp [refineUpdateOpt, refineUpdate] at ref
     have ⟨l, r, span, groups, eqstring, c, eqv⟩ := captureNext.capture_of_some_compile hresH v
-    exact ⟨l, r, span, groups, eqstring, c, ref ▸ eqv.materialize c disj⟩
+    have ⟨m, eql, eqm, eqr⟩ := c.span_eq
+    simp at eql eqm eqr
+    have : span.m.reverse ++ span.r = r := by simp [eqr, ←eqm]
+    exact ⟨l, span.m.reverse, span.r, groups, by rw [←eqstring, Span.toString, eql], by simpa [this, eql] using c, ref ▸ eqv.materialize c disj⟩
   | .none =>
     have := hresH ▸ hresB ▸ captureNext.refines (NFA.compile e) NFA.compile_wf bufferSize it
     simp [refineUpdateOpt] at this
